Auto/Embedding/LamChecker.lean
@@ -11,19 +11,48 @@ namespace Auto.Embedding.Lam
 --   2. `.some` entries may be interspersed with `.none` entries
 structure RTable where
   -- Well-formed formulas, with types
-  wf    : Auto.BinTree (List LamSort × LamTerm × LamSort)
+  wf    : Auto.BinTree (List LamSort × LamSort × LamTerm)
   -- Valid propositions
   valid : Auto.BinTree (List LamSort × LamTerm)
 
-inductive ChkStep (lval : LamValuation) where
-  -- Adds `⟨lctx, t, dest⟩` to `rtable.wf`
-  | wf_of_check
-      (lctx : List LamSort)
-      (t : LamTerm)
-      (dest : Nat) : ChkStep lval
-  | valid_of_interp
-      (p : LamTerm)
-      (h : (LamTerm.interpAsProp lval dfLCtxTy (dfLCtxTerm _) p).down)
-      (dest : Nat) : ChkStep lval
+-- An entry of RTable
+inductive REntry where
+  | none    : REntry
+  | wf      : List LamSort → LamSort → LamTerm → REntry
+  | valid   : List LamSort → LamTerm → REntry
+
+def RTable.addEntry (r : RTable) (n : Nat) : REntry → RTable
+| .none         => r
+| .wf lctx s t  => ⟨r.wf.insert n ⟨lctx, s, t⟩, r.valid⟩
+| .valid lctx t => ⟨r.wf, r.valid.insert n ⟨lctx, t⟩⟩
+
+-- Invariant of `wf`
+def RTable.wfInv
+  (lval : LamValuation.{u})
+  (wf : Auto.BinTree (List LamSort × LamSort × LamTerm)) :=
+  wf.allp (fun ⟨lctx, rty, t⟩ => LamThmWF' lval lctx rty t)
+
+-- Invariant of `valid
+def RTable.validInv
+  (lval : LamValuation.{u})
+  (valid : Auto.BinTree (List LamSort × LamTerm)) :=
+  valid.allp (fun ⟨lctx, t⟩ => LamThmValid lval lctx t)
+
+-- Invariant of `RTable`
+def RTable.inv (lval : LamValuation.{u}) (r : RTable) :=
+  wfInv lval r.wf ∧ validInv lval r.valid
+
+inductive ChkStep where
+  -- Adds `⟨lctx, t, t.lamCheck!⟩` to `rtable.wf`
+  | wfOfCheck (lctx : List LamSort) (t : LamTerm) : ChkStep
+
+def ChkStep.eval (ltv : LamTyVal) (r : RTable) : (cs : ChkStep) → REntry
+| .wfOfCheck lctx t =>
+  match LamTerm.lamCheck? ltv (pushLCtxs lctx dfLCtxTy) t with
+  | .some rty =>
+    match Nat.ble (t.maxLooseBVarSucc) (lctx.length) with
+    | true  => .wf lctx rty t
+    | false => .none
+  | .none => .none
 
 end Auto.Embedding.Lam
