Auto/Lib/OptionExtra.lean
@@ -1,0 +1,7 @@
+namespace Auto
+
+@[always_inline, inline] def Option.allp (p : α → Prop) : Option α → Prop
+  | some a => p a
+  | none   => True
+
+end Auto
